Updates.

FOL/Sub/All/Rec/SubAllRecChangeReplaceFree.lean
@@ -10,69 +10,72 @@ namespace FOL
 open Formula
 
 
-def List.str_max_len :
-  List String → ℕ
-| [] => 0
-| hd :: tl => max hd.length (List.str_max_len tl)
+def finset_var_name_max_len :
+  Finset VarName → ℕ :=
+  Finset.fold (fun x x_1 => max x x_1) 0 (String.length ∘ VarName.toString)
 
-lemma list_str_max_len_mem
-  (s : String)
-  (l : List String)
+
+lemma finset_var_name_max_len_mem
+  (s : VarName)
+  (l : Finset VarName)
   (h1 : s ∈ l) :
-  s.length <= List.str_max_len l :=
+  s.length <= finset_var_name_max_len l :=
   by
-  induction l
-  case nil =>
+  induction l using Finset.induction_on
+  case empty =>
     simp at h1
-  case cons hd tl ih =>
+  case insert hd tl a1 ih =>
     simp at h1
-
-    unfold List.str_max_len
     cases h1
     case inl c1 =>
-      simp only [c1]
+      subst c1
+      unfold finset_var_name_max_len
       simp
     case inr c1 =>
-      trans List.str_max_len tl
-      · exact ih c1
-      · simp
+      unfold finset_var_name_max_len at ih
+      unfold finset_var_name_max_len
+      simp
+      right
+      exact ih c1
+
 
 def variant
-  (s : String)
+  (s : VarName)
   (c : Char)
-  (l : List String) :
-  String :=
+  (l : Finset VarName) :
+  VarName :=
   if h : s ∈ l
   then
-  have : List.str_max_len l + 1 - (String.length s + String.length (Char.toString c)) < List.str_max_len l + 1 - String.length s :=
+  have : finset_var_name_max_len l + 1 - (s.length + String.length (Char.toString c)) < finset_var_name_max_len l + 1 - s.length :=
     by
     have s1 : (Char.toString c).length = 1
     rfl
 
     simp only [s1]
     simp
-    obtain s2 := list_str_max_len_mem s l h
+    obtain s2 := finset_var_name_max_len_mem s l h
     simp only [tsub_lt_tsub_iff_right s2]
     simp
-  variant (s ++ c.toString) c l
+  variant (VarName.mk (s.toString ++ c.toString)) c l
   else s
-  termination_by variant s _ l => List.str_max_len l + 1 - s.length
+  termination_by variant s _ l => finset_var_name_max_len l + 1 - s.length
+
 
 lemma variant_spec
-  (s : String)
+  (s : VarName)
   (c : Char)
-  (l : List String) :
+  (l : Finset VarName) :
   ¬ variant s c l ∈ l :=
   if h : s ∈ l
   then
-  have : List.str_max_len l + 1 - (String.length s + String.length (Char.toString c)) < List.str_max_len l + 1 - String.length s :=
+  have : finset_var_name_max_len l + 1 - (s.length + String.length (Char.toString c)) < finset_var_name_max_len l + 1 - s.length :=
     by
     have s1 : (Char.toString c).length = 1
     rfl
 
     simp only [s1]
     simp
-    obtain s2 := list_str_max_len_mem s l h
+    obtain s2 := finset_var_name_max_len_mem s l h
     simp only [tsub_lt_tsub_iff_right s2]
     simp
   by
@@ -85,165 +88,7 @@ lemma variant_spec
     simp
     simp [if_neg h]
     exact h
-  termination_by variant_spec s _ l => List.str_max_len l + 1 - s.length
-
-
-def Finset.str_max_len :
-  Finset String → ℕ :=
-  Finset.fold (fun x x_1 => max x x_1) 0 String.length
-
-lemma finset_str_max_len_mem
-  (s : String)
-  (l : Finset String)
-  (h1 : s ∈ l) :
-  s.length <= Finset.str_max_len l :=
-  by
-  induction l using Finset.induction_on
-  case empty =>
-    simp at h1
-  case insert hd tl a1 ih =>
-    simp at h1
-    cases h1
-    case inl c1 =>
-      subst c1
-      unfold Finset.str_max_len
-      simp
-    case inr c1 =>
-      unfold Finset.str_max_len at ih
-      unfold Finset.str_max_len
-      simp
-      right
-      exact ih c1
-
-def FinsetVariant
-  (s : String)
-  (c : Char)
-  (l : Finset String) :
-  String :=
-  if h : s ∈ l
-  then
-  have : Finset.str_max_len l + 1 - (String.length s + String.length (Char.toString c)) < Finset.str_max_len l + 1 - String.length s :=
-    by
-    have s1 : (Char.toString c).length = 1
-    rfl
-
-    simp only [s1]
-    simp
-    obtain s2 := finset_str_max_len_mem s l h
-    simp only [tsub_lt_tsub_iff_right s2]
-    simp
-  FinsetVariant (s ++ c.toString) c l
-  else s
-  termination_by FinsetVariant s _ l => Finset.str_max_len l + 1 - s.length
-
-
-lemma variant_spec'
-  (s : String)
-  (c : Char)
-  (l : Finset String) :
-  ¬ FinsetVariant s c l ∈ l :=
-  if h : s ∈ l
-  then
-  have : Finset.str_max_len l + 1 - (String.length s + String.length (Char.toString c)) < Finset.str_max_len l + 1 - String.length s :=
-    by
-    have s1 : (Char.toString c).length = 1
-    rfl
-
-    simp only [s1]
-    simp
-    obtain s2 := finset_str_max_len_mem s l h
-    simp only [tsub_lt_tsub_iff_right s2]
-    simp
-  by
-    unfold FinsetVariant
-    simp
-    simp only [if_pos h]
-    apply variant_spec'
-  else by
-    unfold FinsetVariant
-    simp
-    simp [if_neg h]
-    exact h
-  termination_by variant_spec' s _ l => Finset.str_max_len l + 1 - s.length
-
-
-def Finset.var_name_max_len :
-  Finset VarName → ℕ :=
-  Finset.fold (fun x x_1 => max x x_1) 0 (String.length ∘ VarName.toString)
-
-lemma finset_var_name_max_len_mem
-  (s : VarName)
-  (l : Finset VarName)
-  (h1 : s ∈ l) :
-  s.length <= Finset.var_name_max_len l :=
-  by
-  induction l using Finset.induction_on
-  case empty =>
-    simp at h1
-  case insert hd tl a1 ih =>
-    simp at h1
-    cases h1
-    case inl c1 =>
-      subst c1
-      unfold Finset.var_name_max_len
-      simp
-    case inr c1 =>
-      unfold Finset.var_name_max_len at ih
-      unfold Finset.var_name_max_len
-      simp
-      right
-      exact ih c1
-
-def FinsetVarNameVariant
-  (s : VarName)
-  (c : Char)
-  (l : Finset VarName) :
-  VarName :=
-  if h : s ∈ l
-  then
-  have : Finset.var_name_max_len l + 1 - (s.length + String.length (Char.toString c)) < Finset.var_name_max_len l + 1 - s.length :=
-    by
-    have s1 : (Char.toString c).length = 1
-    rfl
-
-    simp only [s1]
-    simp
-    obtain s2 := finset_var_name_max_len_mem s l h
-    simp only [tsub_lt_tsub_iff_right s2]
-    simp
-  FinsetVarNameVariant (VarName.mk (s.toString ++ c.toString)) c l
-  else s
-  termination_by FinsetVarNameVariant s _ l => Finset.var_name_max_len l + 1 - s.length
-
-
-lemma variant_spec''
-  (s : VarName)
-  (c : Char)
-  (l : Finset VarName) :
-  ¬ FinsetVarNameVariant s c l ∈ l :=
-  if h : s ∈ l
-  then
-  have : Finset.var_name_max_len l + 1 - (s.length + String.length (Char.toString c)) < Finset.var_name_max_len l + 1 - s.length :=
-    by
-    have s1 : (Char.toString c).length = 1
-    rfl
-
-    simp only [s1]
-    simp
-    obtain s2 := finset_var_name_max_len_mem s l h
-    simp only [tsub_lt_tsub_iff_right s2]
-    simp
-  by
-    unfold FinsetVarNameVariant
-    simp
-    simp only [if_pos h]
-    apply variant_spec''
-  else by
-    unfold FinsetVarNameVariant
-    simp
-    simp [if_neg h]
-    exact h
-  termination_by variant_spec'' s _ l => Finset.var_name_max_len l + 1 - s.length
+  termination_by variant_spec s _ l => finset_var_name_max_len l + 1 - s.length
 
 
 def subVariant
@@ -263,13 +108,13 @@ def subVariant
 | forall_ x phi =>
   let x' : VarName :=
     if ∃ (y : VarName), y ∈ phi.freeVarSet \ {x} ∧ x = σ y
-    then FinsetVarNameVariant x c ((subVariant (Function.updateIte σ x x) c phi).freeVarSet)
+    then variant x c ((subVariant (Function.updateIte σ x x) c phi).freeVarSet)
     else x
   forall_ x' (subVariant (Function.updateIte σ x x') c phi)
 | exists_ x phi =>
   let x' : VarName :=
     if ∃ (y : VarName), y ∈ phi.freeVarSet \ {x} ∧ x = σ y
-    then FinsetVarNameVariant x c ((subVariant (Function.updateIte σ x x) c phi).freeVarSet)
+    then variant x c ((subVariant (Function.updateIte σ x x) c phi).freeVarSet)
     else x
   exists_ x' (subVariant (Function.updateIte σ x x') c phi)
 | def_ X xs => def_ X (xs.map σ)
